Prove payloadLang transitions stable under addition/removal of unused bindings

projection/payloadLangScript.sml
@@ -19,4 +19,34 @@ network = NNil
         | NEndpoint proc state endpoint
 `
 
+val var_names_endpoint_def = Define `
+   (var_names_endpoint Nil = [])
+/\ (var_names_endpoint (Send p v n e) = v::var_names_endpoint e)
+/\ (var_names_endpoint (Receive p v d e) = v::var_names_endpoint e)
+/\ (var_names_endpoint (IntChoice b p e) = var_names_endpoint e)
+/\ (var_names_endpoint (ExtChoice p e1 e2) = var_names_endpoint e1 ++ var_names_endpoint e2)
+/\ (var_names_endpoint (IfThen v e1 e2) = v::var_names_endpoint e1 ++ var_names_endpoint e2)
+/\ (var_names_endpoint (Let v f vl e) = v::vl ++ var_names_endpoint e)
+`
+
+val free_var_names_endpoint_def = Define `
+   (free_var_names_endpoint Nil = [])
+/\ (free_var_names_endpoint (Send p v n e) = v::free_var_names_endpoint e)
+/\ (free_var_names_endpoint (Receive p v d e) = FILTER ($≠ v) (free_var_names_endpoint e))
+/\ (free_var_names_endpoint (IntChoice b p e) = free_var_names_endpoint e)
+/\ (free_var_names_endpoint (ExtChoice p e1 e2) = free_var_names_endpoint e1 ++ free_var_names_endpoint e2)
+/\ (free_var_names_endpoint (IfThen v e1 e2) = v::free_var_names_endpoint e1 ++ free_var_names_endpoint e2)
+/\ (free_var_names_endpoint (Let v f vl e) = vl ++ FILTER ($≠ v) (free_var_names_endpoint e))
+`
+
+val var_names_network_def = Define `
+   (var_names_network NNil = [])
+/\ (var_names_network (NEndpoint p s e) = var_names_endpoint e)
+/\ (var_names_network (NPar n1 n2) = var_names_network n1 ++ var_names_network n2)`
+
+val free_var_names_network_def = Define `
+   (free_var_names_network NNil = [])
+/\ (free_var_names_network (NEndpoint p s e) = free_var_names_endpoint e)
+/\ (free_var_names_network (NPar n1 n2) = free_var_names_network n1 ++ free_var_names_network n2)`
+
 val _ = export_theory ()
