projection/proofs/payloadPropsScript.sml
@@ -3,8 +3,6 @@ open preamble payloadSemanticsTheory payloadLangTheory;
 val _ = new_theory "payloadProps"
 
 val (qcong_rules, qcong_ind, qcong_cases) = Hol_reln `
-(* Basic congruence rules *)
-
   (* Reflexive *)
   (∀n. qcong n n)
 
@@ -532,5 +530,393 @@ val reduction_nil = Q.store_thm("reduction_nil",
   >> MAP_EVERY (W(curry Q.SPEC_TAC)) [`n`,`a1`]
   >> ho_match_mp_tac RTC_lifts_invariants
   >> simp[payloadSemanticsTheory.reduction_def,trans_nil_false]);
+
+val (junkcong_rules, junkcong_ind, junkcong_cases) = Hol_reln `
+  (* Reflexive *)
+  (∀fvs n. junkcong fvs n n)
+
+  (* Symmetric *)
+∧ (∀n1 n2 fvs.
+    junkcong fvs n1 n2
+    ⇒ junkcong fvs n2 n1)
+  (* Transitive *)
+∧ (∀n1 n2 n3 fvs.
+     junkcong fvs n1 n2
+     ∧ junkcong fvs n2 n3
+     ⇒ junkcong fvs n1 n3)
+
+  (* Add-junk *)
+∧ (∀p s e v fvs d.
+    v ∈ fvs ∧ ¬MEM v (free_var_names_endpoint e)
+    ⇒ junkcong fvs (NEndpoint p s e) (NEndpoint p (s with bindings:= s.bindings |+ (v,d)) e))
+
+  (* Par *)
+∧ (∀n1 n2 n3 n4 fvs.
+     junkcong fvs n1 n2
+     ∧ junkcong fvs n3 n4
+     ⇒ junkcong fvs (NPar n1 n3) (NPar n2 n4))`
+
+val [junkcong_refl,junkcong_sym,junkcong_trans,junkcong_add_junk,junkcong_par]
+    = zip ["junkcong_refl","junkcong_sym","junkcong_trans","junkcong_add_junk","junkcong_par"]
+          (CONJUNCTS junkcong_rules) |> map save_thm;
+
+val junkcong_strongind = fetch "-" "junkcong_strongind"
+
+val junkcong_refl_IMP = Q.store_thm("junkcong_refl_IMP",
+  `∀fvs n n'. n = n' ==> junkcong fvs n n'`,
+  simp[junkcong_refl]);
+
+val junkcong_add_junk' = Q.store_thm("junkcong_add_junk'",
+ `∀p s b e v fvs d.
+    v ∈ fvs ∧ ¬MEM v (free_var_names_endpoint e)
+    ⇒ junkcong fvs (NEndpoint p (s with bindings := b) e) (NEndpoint p (s with bindings:= b |+ (v,d)) e)`,
+ rpt strip_tac
+ >> `s with bindings := b |+ (v,d) =
+     (s with bindings := b) with bindings := (s with bindings := b).bindings |+ (v,d)`
+      by simp[]
+ >> pop_assum(fn thm => PURE_ONCE_REWRITE_TAC [thm])
+ >> match_mp_tac junkcong_add_junk >> simp[]);
+
+val junkcong_add_junk'' = Q.store_thm("junkcong_add_junk''",
+ `∀p b q e v fvs d.
+    v ∈ fvs ∧ ¬MEM v (free_var_names_endpoint e)
+    ⇒ junkcong fvs (NEndpoint p <|bindings := b; queue := q|> e)
+                    (NEndpoint p <|bindings := b |+ (v,d); queue := q|> e)`,
+ rpt strip_tac
+ >> qmatch_goalsub_abbrev_tac `junkcong _ (NEndpoint _ a1 _) (NEndpoint _ a2 _)`
+ >> `a2 = a1 with bindings := a1.bindings |+ (v,d)`
+     by(unabbrev_all_tac >> simp[])
+ >> rveq
+ >> match_mp_tac junkcong_add_junk >> simp[]);
+
+val junkcong_remove_junk = Q.store_thm("junkcong_remove_junk",
+  `(∀p s e v fvs.
+    v ∈ fvs ∧ ¬MEM v (free_var_names_endpoint e)
+    ⇒ junkcong fvs (NEndpoint p s e) (NEndpoint p (s with bindings:= s.bindings \\ v) e))`,
+  rpt strip_tac
+  >> Cases_on `v ∈ FDOM s.bindings`
+  >- (fs[FDOM_FLOOKUP] >> rename1 `FLOOKUP _ _ = SOME d`
+      >> drule junkcong_add_junk >> disch_then drule
+      >> disch_then (qspecl_then [`p`,`s with bindings := s.bindings \\ v`,`d`] assume_tac)
+      >> fs[GSYM FUPDATE_PURGE]
+      >> `s.bindings |+ (v,d) = s.bindings`
+           by(match_mp_tac FUPDATE_ELIM >> fs[flookup_thm])
+      >> `s with bindings := s.bindings = s` by fs[endpointLangTheory.state_component_equality]
+      >> fs[FUPDATE_ELIM] >> match_mp_tac junkcong_sym >> first_x_assum ACCEPT_TAC)
+  >- (fs[DOMSUB_NOT_IN_DOM]
+      >> match_mp_tac junkcong_refl_IMP >> simp[endpointLangTheory.state_component_equality]));
+
+val junkcong_sym_eq = Q.store_thm("junkcong_sym_eq",
+`∀fvs p q. junkcong fvs p q = junkcong fvs q p`,metis_tac[junkcong_sym]);
+
+val junkcong_trans_eq = Q.store_thm("junkcong_trans_eq",
+  `∀fvs p1 q1.
+     junkcong fvs p1 q1
+     ⇒ ∀ conf alpha p2 q2.
+            ((trans conf p1 alpha p2 ⇒ (∃q2. trans conf q1 alpha q2 ∧ junkcong fvs p2 q2))
+         ∧ (trans conf q1 alpha q2 ⇒ (∃p2. trans conf p1 alpha p2 ∧ junkcong fvs p2 q2)))`,
+  ho_match_mp_tac junkcong_strongind
+  >> rpt strip_tac
+  >- metis_tac[junkcong_rules]
+  >- metis_tac[junkcong_rules]
+  >- metis_tac[junkcong_rules]
+  >- metis_tac[junkcong_rules]
+  >- metis_tac[junkcong_rules]
+  >- metis_tac[junkcong_rules]
+  >- (* junkcong_add_junk *)
+     (qpat_x_assum `trans _ _ _ _` (assume_tac
+                                    o REWRITE_RULE [Once payloadSemanticsTheory.trans_cases])
+      >> fs[] >> rveq
+      >> TRY(qmatch_goalsub_abbrev_tac `junkcong fvs (NEndpoint a1 a2 a3)`
+             >> qexists_tac `NEndpoint a1 (a2 with bindings := a2.bindings |+ (v,d)) a3`
+             >> conj_tac
+             >- (unabbrev_all_tac
+                 >> MAP_FIRST match_mp_tac (CONJUNCTS payloadSemanticsTheory.trans_rules)
+                 >> fs[FLOOKUP_UPDATE,free_var_names_endpoint_def])
+             >- (`¬MEM v (free_var_names_endpoint a3)`
+                   by(unabbrev_all_tac >> fs[free_var_names_endpoint_def])
+                 >> fs[free_var_names_endpoint_def] >> metis_tac[junkcong_rules]))
+      >> TRY(qmatch_goalsub_abbrev_tac `junkcong fvs (NEndpoint a1 (a2 with queue := a3) a4)`
+             >> qexists_tac `NEndpoint a1 (a2 with <|queue := a3; bindings := a2.bindings |+ (v,d)|>) a4`
+             >> conj_tac
+             >- (PURE_ONCE_REWRITE_TAC [endpointLangTheory.state_fupdcanon]
+                 >> qmatch_goalsub_abbrev_tac `trans _ (NEndpoint _ a5 _)`
+                 >> `a2 with <|bindings := a2.bindings |+ (v,d); queue := a3|>
+                     = a5 with queue := a3` by(unabbrev_all_tac >> simp[])
+                 >> pop_assum (fn thm => PURE_ONCE_REWRITE_TAC[thm])
+                 >> qunabbrev_tac `a3`
+                 >> `a2.queue = a5.queue` by(unabbrev_all_tac >> simp[])
+                 >> pop_assum (fn thm => PURE_ONCE_REWRITE_TAC[thm])
+                 >> MAP_FIRST match_mp_tac (CONJUNCTS trans_rules)
+                 >> simp[])
+             >- (imp_res_tac junkcong_add_junk
+                 >> pop_assum(qspec_then `a2 with queue := a3` assume_tac)
+                 >> fs[]))
+      >> TRY(qmatch_goalsub_abbrev_tac `junkcong fvs (NEndpoint a1
+                                                                <|bindings := a2;
+                                                                  queue := a3|>
+                                                                a4)`
+             >> qexists_tac `NEndpoint a1 <|bindings := if v = v' then a2
+                                                        else a2 |+ (v,d); queue := a3|> a4`
+             >> conj_tac
+             >- (IF_CASES_TAC
+                 >> unabbrev_all_tac
+                 >> `s.queue = (s with bindings := s.bindings |+ (v,d)).queue` by simp[]
+                 >> pop_assum(fn thm => FULL_SIMP_TAC bool_ss [Once thm])
+                 >> imp_res_tac trans_dequeue_last_payload
+                 >> first_x_assum(qspec_then `v'` assume_tac)
+                 >> rveq                     
+                 >> fs[Once FUPDATE_COMMUTES])
+             >- (IF_CASES_TAC
+                 >- metis_tac[junkcong_rules]
+                 >> `¬MEM v (free_var_names_endpoint a4)`
+                     by(unabbrev_all_tac >> fs[free_var_names_endpoint_def,MEM_FILTER])
+                 >> metis_tac[junkcong_add_junk'']))
+      >> TRY(qmatch_goalsub_abbrev_tac `junkcong fvs (NEndpoint a1 (a2 with queue := a3) a4)`
+             >> qexists_tac `NEndpoint a1 (<|queue := a3;
+                                             bindings := a2.bindings |+ (v,d)|>) a4`
+             >> conj_tac
+             >- (PURE_ONCE_REWRITE_TAC [endpointLangTheory.state_fupdcanon]
+                 >> qmatch_goalsub_abbrev_tac `trans _ (NEndpoint _ a5 _)`
+                 >> `<|bindings := a2.bindings |+ (v,d); queue := a3|>
+                     = a5 with queue := a3` by(unabbrev_all_tac >> simp[])
+                 >> pop_assum (fn thm => PURE_ONCE_REWRITE_TAC[thm])
+                 >> qunabbrev_tac `a4`
+                 >> qunabbrev_tac `a3`
+                 >> `a2.queue = a5.queue` by(unabbrev_all_tac >> simp[])
+                 >> pop_assum (fn thm => PURE_ONCE_REWRITE_TAC[thm])
+                 >> MAP_FIRST match_mp_tac (CONJUNCTS trans_rules)
+                 >> unabbrev_all_tac >> simp[])
+             >- (`¬MEM v (free_var_names_endpoint a4)`
+                   by(unabbrev_all_tac >> fs[free_var_names_endpoint_def])
+                 >> imp_res_tac junkcong_add_junk
+                 >> rpt(first_x_assum(qspec_then `a2 with queue := a3` assume_tac ))
+                 >> fs[]))
+      >> TRY(qmatch_goalsub_abbrev_tac `junkcong fvs (NEndpoint a1 (a2 with bindings := a3) a4)`
+             >> qexists_tac `NEndpoint a1 (a2 with bindings := if v = v' then a3
+                                                               else a3|+ (v,d)) a4`
+             >> conj_tac
+             >- (IF_CASES_TAC
+                 >> unabbrev_all_tac >> fs[free_var_names_endpoint_def,MEM_FILTER]
+                 >> `EVERY IS_SOME (MAP (FLOOKUP ((s with bindings := s.bindings |+ (v,d)).bindings)) vl)`
+                     by(fs[EVERY_MAP,FLOOKUP_UPDATE,EVERY_MEM] >> rw[])
+                 >> drule trans_let >> fs[] >> disch_then(qspecl_then [`conf`,`v'`] assume_tac)
+                 >> `MAP (THE ∘ FLOOKUP (s.bindings |+ (v,d))) vl
+                     = MAP (THE ∘ FLOOKUP s.bindings) vl`
+                     by(rw[MAP_EQ_f,FLOOKUP_UPDATE] >> rw[] >> fs[])
+                 >> rfs[] >> fs[Once FUPDATE_COMMUTES])
+             >- (IF_CASES_TAC
+                 >- metis_tac[junkcong_rules]
+                 >- (match_mp_tac junkcong_add_junk' >> fs[free_var_names_endpoint_def,MEM_FILTER])))
+     )
+  >- (* junkcong_add_junk, symmetric case *)
+     (PURE_ONCE_REWRITE_TAC [junkcong_sym_eq]
+      >> qpat_x_assum `trans _ _ _ _` (assume_tac
+                                       o REWRITE_RULE [Once payloadSemanticsTheory.trans_cases])
+      >> fs[] >> rveq
+      >> TRY(qmatch_goalsub_abbrev_tac `junkcong fvs (NEndpoint a1 (a2 with bindings := _) a3)`
+             >> qexists_tac `NEndpoint a1 a2 a3`
+             >> conj_tac
+             >- (unabbrev_all_tac
+                 >> MAP_FIRST match_mp_tac (CONJUNCTS payloadSemanticsTheory.trans_rules)
+                 >> fs[FLOOKUP_UPDATE,free_var_names_endpoint_def] >> rfs[])
+             >- (`¬MEM v (free_var_names_endpoint a3)`
+                   by(unabbrev_all_tac >> fs[free_var_names_endpoint_def])
+                 >> fs[free_var_names_endpoint_def] >> metis_tac[junkcong_rules]))
+      >> TRY(qmatch_goalsub_abbrev_tac `junkcong fvs
+                                                (NEndpoint a1
+                                                           <|bindings := a2 |+ _ |+ (a3,a4);
+                                                             queue := a5|> a6)`
+             >> qexists_tac `NEndpoint a1 (s with <|queue := a5; bindings := a2 |+ (a3,a4)|>) a6`
+             >> conj_tac
+             >- (unabbrev_all_tac >> MAP_FIRST match_mp_tac (CONJUNCTS trans_rules)
+                 >> simp[])
+             >- (Cases_on `v = a3` >> fs[Once FUPDATE_COMMUTES]
+                 >> fs[free_var_names_endpoint_def,MEM_FILTER]
+                 >> metis_tac[junkcong_rules,junkcong_add_junk']))      
+      >> TRY(qmatch_goalsub_abbrev_tac `junkcong fvs
+                                                (NEndpoint a1
+                                                           <|bindings := a2 |+ (v,d);
+                                                             queue := a3|> a4)`
+             >> qexists_tac `NEndpoint a1 (s with queue := a3) a4`
+             >> conj_tac
+             >- (PURE_ONCE_REWRITE_TAC [endpointLangTheory.state_fupdcanon]
+                 >> unabbrev_all_tac
+                 >> MAP_FIRST match_mp_tac (CONJUNCTS trans_rules)
+                 >> simp[])
+             >- (`¬MEM v (free_var_names_endpoint a4)`
+                   by(unabbrev_all_tac >> fs[free_var_names_endpoint_def])
+                 >> imp_res_tac junkcong_add_junk
+                 >> rpt(first_x_assum(qspec_then `s with queue := a3` assume_tac))
+                 >> fs[] >> rw[Once junkcong_sym_eq] >> unabbrev_all_tac >> fs[]))
+      >> TRY(qmatch_goalsub_abbrev_tac `junkcong fvs
+                                                 (NEndpoint a1
+                                                            (s with bindings := a2 |+ _ |+ (a3,a4))
+                                                            a5)`
+             >> qexists_tac `NEndpoint a1 (s with bindings := a2 |+ (a3,a4)) a5`
+             >> conj_tac
+             >- (unabbrev_all_tac >> fs[free_var_names_endpoint_def,MEM_FILTER]
+                 >> `MAP (THE ∘ FLOOKUP (s.bindings |+ (v,d))) vl
+                     = MAP (THE ∘ FLOOKUP s.bindings) vl`
+                      by(rw[MAP_EQ_f,FLOOKUP_UPDATE] >> rw[] >> fs[])
+                 >> fs[] >> match_mp_tac trans_let >> fs[EVERY_MAP,EVERY_MEM] >> rw[]
+                 >> first_x_assum drule >> strip_tac >> fs[IS_SOME_EXISTS,FLOOKUP_UPDATE]
+                 >> every_case_tac >> fs[])
+             >- (Cases_on `a3 = v` >> fs[Once FUPDATE_COMMUTES]
+                 >> fs[free_var_names_endpoint_def,MEM_FILTER]
+                 >> metis_tac[junkcong_rules,junkcong_add_junk'])))
+  >- (* par-l *)
+     (qpat_x_assum `trans _ (NPar _ _) _ _` (assume_tac
+                                    o REWRITE_RULE [Once payloadSemanticsTheory.trans_cases])
+      >> fs[] >> rveq
+      >> EVERY_ASSUM imp_res_tac
+      >> imp_res_tac trans_com_l
+      >> imp_res_tac trans_com_r
+      >> imp_res_tac trans_com_choice_l
+      >> imp_res_tac trans_com_choice_r
+      >> imp_res_tac trans_par_l
+      >> imp_res_tac trans_par_r
+      >> metis_tac[junkcong_rules])
+  >- (* par-r *)
+     (qpat_x_assum `trans _ (NPar _ _) _ _` (assume_tac
+                                    o REWRITE_RULE [Once payloadSemanticsTheory.trans_cases])
+      >> fs[] >> rveq
+      >> EVERY_ASSUM imp_res_tac
+      >> imp_res_tac trans_com_l
+      >> imp_res_tac trans_com_r
+      >> imp_res_tac trans_com_choice_l
+      >> imp_res_tac trans_com_choice_r
+      >> imp_res_tac trans_par_l
+      >> imp_res_tac trans_par_r
+      >> metis_tac[junkcong_rules]));
+
+val junkcong_trans_pres = Q.store_thm("junkcong_trans_pres",
+  `∀p1 q1 fv conf alpha p2.
+     junkcong fv p1 q1 ∧ trans conf p1 alpha p2
+     ⇒ ∃q2. trans conf q1 alpha q2 ∧ junkcong fv p2 q2`,
+  metis_tac[junkcong_trans_eq])
+
+val reduction_par_l = Q.store_thm("reduction_par_l",
+  `∀p q r conf. (reduction conf)^* p q ==> (reduction conf)^* (NPar p r) (NPar q r)`,
+  rpt gen_tac
+  >> MAP_EVERY (W(curry Q.SPEC_TAC)) [`q`,`p`]
+  >> ho_match_mp_tac RTC_INDUCT
+  >> rpt strip_tac
+  >- simp[RTC_REFL]
+  >> match_mp_tac (RTC_RULES |> SPEC_ALL |> CONJUNCT2)
+  >> metis_tac[reduction_def,trans_par_l]);
+
+val reduction_par_r = Q.store_thm("reduction_par_r",
+  `∀p q r conf. (reduction conf)^* p q ==> (reduction conf)^* (NPar r p) (NPar r q)`,
+  rpt gen_tac
+  >> MAP_EVERY (W(curry Q.SPEC_TAC)) [`q`,`p`]
+  >> ho_match_mp_tac RTC_INDUCT
+  >> rpt strip_tac
+  >- simp[RTC_REFL]
+  >> match_mp_tac (RTC_RULES |> SPEC_ALL |> CONJUNCT2)
+  >> metis_tac[reduction_def,trans_par_r]);
+
+val trans_nil_false = Q.store_thm("trans_nil_false",
+  `∀conf alpha n. trans conf NNil alpha n = F`,
+  rpt strip_tac
+  >> PURE_ONCE_REWRITE_TAC[trans_cases]
+  >> fs[]);
+
+val reduction_nil = Q.store_thm("reduction_nil",
+  `∀conf n. (reduction conf)^* NNil n ==> n = NNil`,
+  rpt strip_tac
+  >> qpat_abbrev_tac `a1 = NNil`
+  >> pop_assum (assume_tac o REWRITE_RULE[markerTheory.Abbrev_def])
+  >> simp[]
+  >> rpt(last_x_assum mp_tac)
+  >> PURE_ONCE_REWRITE_TAC [AND_IMP_INTRO]
+  >> MAP_EVERY (W(curry Q.SPEC_TAC)) [`n`,`a1`]
+  >> ho_match_mp_tac RTC_lifts_invariants
+  >> simp[payloadSemanticsTheory.reduction_def,trans_nil_false]);
+
+val list_trans_def = Define `
+    (list_trans conf p [] q = (p = q))
+ /\ (list_trans conf p (alpha::l) q = ?p'. trans conf p alpha p' /\ list_trans conf p' l q)`
+
+val list_trans_append = Q.store_thm("list_trans_append",
+  `!l1 n1 l2 n2 conf. list_trans conf n1 (l1 ++ l2) n2 =
+  ?n3. list_trans conf n1 l1 n3 /\ list_trans conf n3 l2 n2`,
+  Induct_on `l1` >> rpt strip_tac >> fs[list_trans_def]
+  >> rw[EQ_IMP_THM] >> fs[] >> metis_tac[]);
+
+val list_trans_par_l = Q.store_thm("list_trans_par_l",
+  `∀conf p alpha q r. list_trans conf p alpha q ==> list_trans conf (NPar p r) alpha (NPar q r)`,
+  Induct_on `alpha`
+  >- simp[list_trans_def]
+  >> rpt strip_tac
+  >> fs[list_trans_def] >> metis_tac[payloadSemanticsTheory.trans_par_l]);
+
+val list_trans_par_r = Q.store_thm("list_trans_par_r",
+  `∀conf p alpha q r. list_trans conf p alpha q ==> list_trans conf (NPar r p) alpha (NPar r q)`,
+  Induct_on `alpha`
+  >- simp[list_trans_def]
+  >> rpt strip_tac
+  >> fs[list_trans_def] >> metis_tac[payloadSemanticsTheory.trans_par_r]);
+
+val endpoints_def = Define `
+   (endpoints NNil = [])
+/\ (endpoints (NEndpoint p1 s e1) = [(p1,s,e1)])
+/\ (endpoints (NPar n1 n2) = endpoints n1 ++ endpoints n2)`
+
+val endpoint_names_trans = Q.store_thm("endpoint_names_trans",
+  `!conf n1 alpha n2. trans conf n1 alpha n2 ==> MAP FST (endpoints n2) = MAP FST(endpoints n1)`,
+  ho_match_mp_tac trans_strongind >> rpt strip_tac >> fs[endpoints_def]);
+
+val sender_is_endpoint = Q.store_thm("sender_is_endpoint",
+ `∀p1 p2 q1 d q2 conf.
+  trans conf p1 (LSend q1 d q2) p2 ==> MEM q1 (MAP FST (endpoints p1))`,
+  rpt strip_tac
+  >> qmatch_asmsub_abbrev_tac `trans _ _ alpha _`
+  >> pop_assum (mp_tac o REWRITE_RULE[markerTheory.Abbrev_def])
+  >> MAP_EVERY (W(curry Q.SPEC_TAC)) [`q1`,`d`,`q2`]
+  >> pop_assum mp_tac
+  >> MAP_EVERY (W(curry Q.SPEC_TAC)) [`p2`,`alpha`,`p1`,`conf`]
+  >> ho_match_mp_tac trans_strongind
+  >> rpt strip_tac >> fs[] >> rveq
+  >> fs[endpoints_def]);
+
+val choice_sender_is_endpoint = Q.store_thm("choice_sender_is_endpoint",
+ `∀p1 p2 q1 d q2 conf.
+  trans conf p1 (LIntChoice q1 d q2) p2 ==> MEM q1 (MAP FST (endpoints p1))`,
+  rpt strip_tac
+  >> qmatch_asmsub_abbrev_tac `trans _ _ alpha _`
+  >> pop_assum (mp_tac o REWRITE_RULE[markerTheory.Abbrev_def])
+  >> MAP_EVERY (W(curry Q.SPEC_TAC)) [`q1`,`d`,`q2`]
+  >> pop_assum mp_tac
+  >> MAP_EVERY (W(curry Q.SPEC_TAC)) [`p2`,`alpha`,`p1`,`conf`]
+  >> ho_match_mp_tac trans_strongind
+  >> rpt strip_tac >> fs[] >> rveq
+  >> fs[endpoints_def]);
+
+val choice_receiver_is_endpoint = Q.store_thm("choice_receiver_is_endpoint",
+ `∀p1 p2 q1 d q2 conf.
+  trans conf p1 (LExtChoice q1 d q2) p2 ==> MEM q2 (MAP FST (endpoints p1))`,
+  rpt strip_tac
+  >> qmatch_asmsub_abbrev_tac `trans _ _ alpha _`
+  >> pop_assum (mp_tac o REWRITE_RULE[markerTheory.Abbrev_def])
+  >> MAP_EVERY (W(curry Q.SPEC_TAC)) [`q1`,`d`,`q2`]
+  >> pop_assum mp_tac
+  >> MAP_EVERY (W(curry Q.SPEC_TAC)) [`p2`,`alpha`,`p1`,`conf`]
+  >> ho_match_mp_tac trans_strongind
+  >> rpt strip_tac >> fs[] >> rveq
+  >> fs[endpoints_def]);
+
+val receiver_is_endpoint = Q.store_thm("receiver_is_endpoint",
+ `∀p1 p2 q1 d q2 conf.
+  trans conf p1 (LReceive q1 d q2) p2 ==> MEM q2 (MAP FST (endpoints p1))`,
+  rpt strip_tac
+  >> qmatch_asmsub_abbrev_tac `trans _ _ alpha _`
+  >> pop_assum (mp_tac o REWRITE_RULE[markerTheory.Abbrev_def])
+  >> MAP_EVERY (W(curry Q.SPEC_TAC)) [`q1`,`d`,`q2`]
+  >> pop_assum mp_tac
+  >> MAP_EVERY (W(curry Q.SPEC_TAC)) [`p2`,`alpha`,`p1`,`conf`]
+  >> ho_match_mp_tac trans_strongind
+  >> rpt strip_tac >> fs[] >> rveq
+  >> fs[endpoints_def]);
 
 val _ = export_theory ()
